demo/testc.thy
@@ -1,0 +1,24 @@
+theory testc
+imports Main
+        "../IsaHipster"
+begin
+
+datatype Nat = Z | S Nat
+
+fun le :: "Nat => Nat => bool" where
+  "le Z     y      = True"
+| "le y Z      = False"
+| "le (S z) (S x2) = le z x2"
+
+fun eqN :: "Nat => Nat => bool" where
+  "eqN Z      Z    = True"
+| "eqN Z     (S z) = False"
+| "eqN (S x)  Z    = False"
+| "eqN (S x) (S y) = eqN x y"
+
+setup{*Hip_Tac_Ops.toggle_full_types @{context}*}
+setup{*Hip_Tac_Ops.set_metis_to @{context} 1000*}
+
+hipster_cond le
+
+end
